cava/arrow-examples/Aes/Util.v
@@ -26,60 +26,58 @@ match n with
   ]>
 end.
 
-Fixpoint map2_xor {n}
-  : kappa_sugared var << Vector (S n) Bit, Vector (S n) Bit, Unit >> <<Vector (S n) Bit>> :=
+Fixpoint map {n T}
+  (f : kappa_sugared var <<T, Unit>> T)
+  : kappa_sugared var << Vector (S n) T, Unit >> <<Vector (S n) T>> :=
 match n with
-| 0 => <[ \x y => mkVec (xor (x[#0]) (y[#0])) ]> 
+| 0 => <[ \x => mkVec (!f (x[#0])) ]> 
+| S n' =>
+  <[ \xs =>
+      let '(x, xs') = !kappa_head' xs in
+      !f x :: (!(@map n' _ f) xs') 
+  ]> 
+end.
+
+Fixpoint map2 {n T}
+  (f : kappa_sugared var <<T, T, Unit>> T)
+  : kappa_sugared var << Vector (S n) T, Vector (S n) T, Unit >> <<Vector (S n) T>> :=
+match n with
+| 0 => <[ \x y => mkVec (!f (x[#0]) (y[#0])) ]> 
 | S n' =>
   <[ \xs ys =>
       let '(x, xs') = !kappa_head' xs in
       let '(y, ys') = !kappa_head' ys in
-      concat
-        (mkVec ( xor x y ))
-        (!(@map2_xor n') xs' ys')
+      !f x y :: (!(@map2 n' _ f) xs' ys') 
   ]> 
 end.
 
+Definition map2_xor {n}
+  : kappa_sugared var << Vector (S n) Bit, Vector (S n) Bit, Unit >> <<Vector (S n) Bit>> :=
+  map2 Xor.
+
+Definition map2_xnor {n}
+  : kappa_sugared var << Vector (S n) Bit, Vector (S n) Bit, Unit >> <<Vector (S n) Bit>> :=
+  map2 Xnor.
+
+Definition bitvec_eq {n}
+  : kappa_sugared var << Vector (S n) Bit, Vector (S n) Bit, Unit >> <<Bit>> :=
+  <[\ x y => !(reduce And) (!map2_xnor x y) ]>.
+
+Definition enable_vec {n}
+  : kappa_sugared var << Bit, Vector (S n) Bit, Unit >> <<Vector (S n) Bit>> :=
+  <[\ enable xs => !(map (App And (Var enable))) xs ]>.
+
+Definition mux_vec {n}
+  : kappa_sugared var << Bit, Vector (S n) Bit, Vector (S n) Bit, Unit >> <<Vector (S n) Bit>> :=
+  <[\ switch xs ys => 
+    let not_switch = not switch
+    in !(map2 Or) (!enable_vec switch xs) (!enable_vec not_switch ys)
+    ]>.
+
 End var.
 
+
 Notation "a ^ b" := (App (App (map2_xor _) a) b) (in custom expr at level 5, left associativity) : kappa_scope.
-
-
-(* Lemma reduce_wf: forall n i (f: Kappa_sugared <<i,i,Unit>> i), 
-  wf_debrujin ENil (Desugar f _) ->
-  wf_debrujin ENil (Desugar (fun var => @reduce var n _ (f _)) _).
-Proof.
-  induction n.
-
-  intros.
-  eapply (@kappa_wf _ _ nil%list).
-  repeat (constructor;intros).
-  simpl.
-  tauto.
-
-  intros.
-  eapply (@kappa_wf _ _ nil%list).
-  repeat (constructor;intros).
-
-  eapply (@kappa_wf _ _ nil%list) in H.
-  Qed. *)
-
-Ltac mk_constructive := 
-  match goal with 
-  | [ H1: Kappa_sugared ?I ?O 
-    , H2: wf_debrujin ENil ((Kappa_sugared ?I ?O) natvar)
-        |- _] =>
-      pose proof (to_constructive (Desugar H1) H2) as x;
-      clear H1; clear H2
-  end.
-
-Ltac show_is_combinational x x_wf := 
-  match goal with 
-  | [H: structure ?I ?O |- _] => 
-    let no_loops_x := fresh "no_loops" in (
-      pose proof (toCava H NoLoops) as no_loops_x;
-      let no_delays_x := fresh "no_delays" in (
-        pose proof (toCava H NoDelays) as no_delays_x
-      )
-    )
-  end.
+Notation "a & b" := (App (App (map2 _ And) a) b) (in custom expr at level 5, left associativity) : kappa_scope.
+Notation "a == b" := (App (App (bitvec_eq _) a) b) (in custom expr at level 5, left associativity) : kappa_scope.
+Notation "'if' i 'then' t 'else' e" := (App (App (App (mux_vec _) i) t) e) (in custom expr at level 5, left associativity) : kappa_scope.
